generic/Zeta.Generic.Interleave.fst
@@ -11,23 +11,34 @@ let idxn_has_prefix_prop (#vspec:_) (#n:nat) (#b:_) (tfn: T.idxfn_t vspec b)
 
 let idxfn_prefix_property (#vspec:_) (#n:_) (#b:_) (tfn: T.idxfn_t vspec b)
   (il: verifiable_log vspec n) (j:nat{j <= S.length il}) (i: nat{i < j})
-  : Lemma (ensures (idxfn tfn il i = idxfn tfn (prefix il j) i))
+  : Lemma (ensures (idxfn tfn il i == idxfn tfn (prefix il j) i))
+  = admit()
+
+let idxfnil_prefix_property (#vspec:_) (#n:_) (#b:eqtype) (tfn: T.idxfn_t vspec b)
+  (il: verifiable_log vspec n) (j:nat{j <= S.length il}) (i: nat{i < j})
+  : Lemma (ensures (idxfn_il tfn il i == idxfn_il tfn (prefix il j) i))
   = admit()
 
 let cond_idxfn_has_prefix_prop (#vspec #n #b #f:_) (m: T.cond_idxfn_t b f)
   : Lemma (ensures (IF.cond_prefix_property #(gen_seq vspec n) #_ #(idxfn f) (cond_idxfn_base m)))
   = admit()
 
-(*
-  let gs = gen_seq vspec n in
-    //let b = timestamp in
-    let f: IF.idxfn_t gs _ = clock #vspec #n in
-    let s: gs.seq_t = il in
-    //assert(IF.prefix_property f);
-    //assert(j <= gs.length s);
-    //assert(i < j);
-    assert(f s i = f (gs.prefix s j) i);
-    //assert(f s i = clock il i);
-    //assert(f (gs.prefix s j) i = clock (prefix il j) i);
-    ()
-    *)
+let lemma_filter_map (#vspec #n:_) (#b:eqtype) (#f:_) (m: T.cond_idxfn_t b f)
+    (il: verifiable_log vspec n) (i: seq_index il)
+  : Lemma (ensures (let fmil = to_fm (cond_idxfn_il #vspec #n #_ #_ m) in
+                    let ilb = IF.filter_map fmil il in
+                    let fm = to_fm m in
+                    let ssb = SF.filter_map (G.gen_sseq vspec) fm (to_glog il) in
+                    let fmil2 = to_fm (cond_idxfn #vspec #n #_ #_ m) in
+                    let sb = IF.filter_map fmil2 il in
+                    ssb = s_seq ilb /\
+                    sb = i_seq ilb))
+  = admit()
+
+let thread_state_pre (#vspec: verifier_spec) (#n:_) (tid:nat{tid < n})
+  : IF.idxfn_t (gen_seq vspec n) (v:vspec.vtls_t {vspec.valid v})
+  = admit()
+
+let thread_state_post (#vspec: verifier_spec) (#n:_) (tid:nat{tid < n})
+  : IF.idxfn_t (gen_seq vspec n) (v:vspec.vtls_t {vspec.valid v})
+  = admit()
