generic/Zeta.Generic.Interleave.fsti
@@ -64,24 +64,24 @@ let idxfn #b #vspec #n (tfn: T.idxfn_t vspec b)
   : IF.idxfn_t (gen_seq vspec n) _
   = idxfn_base tfn
 
-let idxfn_il_base #vspec #n #b (tfn: T.idxfn_t vspec b)
+let idxfn_il_base #vspec #n (#b:eqtype) (tfn: T.idxfn_t vspec b)
   (il: verifiable_log vspec n) (i: seq_index il)
   : elem_src b n
   = {e = idxfn tfn il i; s = src il i}
 
-let idxfn_il #b #vspec #n (tfn: T.idxfn_t vspec b)
+let idxfn_il (#b:eqtype) #vspec #n (tfn: T.idxfn_t vspec b)
   : IF.idxfn_t (gen_seq vspec n) _
   = idxfn_il_base tfn
 
 (* this should be =() proof but does not work since some pattern matching does not kick-in *)
 val idxfn_prefix_property (#vspec:_) (#n:_) (#b:_) (tfn: T.idxfn_t vspec b)
   (il: verifiable_log vspec n) (j:nat{j <= S.length il}) (i: nat{i < j})
-  : Lemma (ensures (idxfn tfn il i = idxfn tfn (prefix il j) i))
+  : Lemma (ensures (idxfn tfn il i == idxfn tfn (prefix il j) i))
           [SMTPat (idxfn tfn (prefix il j) i)]
 
-val idxfnil_prefix_property (#vspec:_) (#n:_) (#b:_) (tfn: T.idxfn_t vspec b)
+val idxfnil_prefix_property (#vspec:_) (#n:_) (#b:eqtype) (tfn: T.idxfn_t vspec b)
   (il: verifiable_log vspec n) (j:nat{j <= S.length il}) (i: nat{i < j})
-  : Lemma (ensures (idxfn_il tfn il i = idxfn_il tfn (prefix il j) i))
+  : Lemma (ensures (idxfn_il tfn il i == idxfn_il tfn (prefix il j) i))
           [SMTPat (idxfn_il tfn (prefix il j) i)]
 
 let cond_idxfn_base #vspec #n #b #f (m: T.cond_idxfn_t b f)
@@ -96,16 +96,16 @@ let cond_idxfn (#vspec #n #b #f:_) (m: T.cond_idxfn_t b f)
   : IF.cond_idxfn_t b (idxfn f)
   = cond_idxfn_base #vspec #n m
 
-let cond_idxfn_il_base #vspec #n #b #f (m: T.cond_idxfn_t b f)
+let cond_idxfn_il_base #vspec #n (#b:eqtype) #f (m: T.cond_idxfn_t b f)
   (il: verifiable_log vspec n) (i: seq_index il{idxfn f il i})
   : elem_src b n
   = {e = cond_idxfn m il i; s = src il i}
 
-let cond_idxfn_il #vspec #n #b #f (m: T.cond_idxfn_t b f)
+let cond_idxfn_il #vspec #n (#b:eqtype) #f (m: T.cond_idxfn_t b f)
   : IF.cond_idxfn_t (elem_src b n) (idxfn f)
   = cond_idxfn_il_base #vspec #n #b #f m
 
-val lemma_filter_map (#vspec #n #b #f:_) (m: T.cond_idxfn_t b f)
+val lemma_filter_map (#vspec #n:_) (#b:eqtype) (#f:_) (m: T.cond_idxfn_t b f)
     (il: verifiable_log vspec n) (i: seq_index il)
   : Lemma (ensures (let fmil = to_fm (cond_idxfn_il #vspec #n #_ #_ m) in
                     let ilb = IF.filter_map fmil il in
@@ -120,4 +120,24 @@ val lemma_filter_map (#vspec #n #b #f:_) (m: T.cond_idxfn_t b f)
 let clock #vspec #n = idxfn #_ #vspec #n (T.clock #vspec)
 
 (* sequence of appfn calls and their results upto epoch ep in the interleaved sequence *)
-let to_appfn_call_res #vspec #n (ep: epoch) = cond_idxfn #vspec #n #_ #_ (T.to_appfn_call_res #vspec ep)
+let to_appfn_call_res #vspec #n = cond_idxfn #vspec #n #_ #_ (T.to_appfn_call_res #vspec)
+
+val thread_state_pre (#vspec: verifier_spec) (#n:_) (tid:nat{tid < n})
+  : IF.idxfn_t (gen_seq vspec n) (v:vspec.vtls_t {vspec.valid v})
+
+val thread_state_post (#vspec: verifier_spec) (#n:_) (tid:nat{tid < n})
+  : IF.idxfn_t (gen_seq vspec n) (v:vspec.vtls_t {vspec.valid v})
+
+let cur_thread_state_pre (#vspec: verifier_spec) (#n:_) (il: verifiable_log vspec n) (i: seq_index il)
+  = let s = src il i in
+    thread_state_pre s il i
+
+let cur_thread_state_post (#vspec: verifier_spec) (#n:_)
+  (il: verifiable_log vspec n) (i: seq_index il)
+  = let s = src il i in
+    thread_state_post s il i
+
+let appfn_calls (#vspec: verifier_spec) (#n:_) (il: verifiable_log vspec n)
+  : seq (Zeta.AppSimulate.appfn_call_res vspec.app)
+  = let fm = IF.to_fm to_appfn_call_res in
+    IF.filter_map fm il
