high2/Zeta.High.Interleave.fsti
@@ -1,8 +1,54 @@
 module Zeta.High.Interleave
 
+open FStar.Seq
 open Zeta.App
 open Zeta.Generic.Interleave
 open Zeta.High.Verifier
+open Zeta.EAC
+
+module V = Zeta.GenericVerifier
+module T = Zeta.Generic.Thread
+module G = Zeta.Generic.Global
+module GI = Zeta.Generic.Interleave
+module I = Zeta.Interleave
+module S = FStar.Seq
+module SA = Zeta.SeqAux
+module IF = Zeta.IdxFn
+module SF = Zeta.SIdxFn
+module EAC=Zeta.EAC
 
 let ilog (app: app_params) = Zeta.Generic.Interleave.ilog (high_verifier_spec app)
 
+let gen_seq (app: app_params)
+  = Zeta.Generic.Interleave.gen_seq (high_verifier_spec app)
+
+let verifiable_log (app:_) (n:nat)
+  = il:ilog app n {verifiable il}
+
+val mk_vlog_entry_ext (#app: app_params) (#n:nat)
+  : IF.idxfn_t (gen_seq app n) (vlog_entry_ext app)
+
+let vlog_ext_of_il_log (#app: app_params) (#n:nat)
+  (il: verifiable_log app n)
+  : seq (vlog_entry_ext app)
+  = IF.map mk_vlog_entry_ext il
+
+let is_eac #app #n (il: verifiable_log app n)
+  = eac (vlog_ext_of_il_log il)
+
+let eac_log (app: app_params) (n:nat) = il: verifiable_log app n {is_eac il}
+
+let neac_log (app: app_params) (n:nat) = il: verifiable_log app n {~ (is_eac il)}
+
+val eac_boundary (#app #n:_) (il: verifiable_log app n)
+  : (i: seq_index il{is_eac (prefix il i) /\
+                     ~ (is_eac (prefix il (i+1)))})
+
+val lemma_eac_implies_prefix_eac (#app #n:_) (il: eac_log app n) (i: nat{i <= S.length il})
+  : Lemma (ensures (is_eac (prefix il i)))
+
+(*val lemma_eac_implies_appfn_valid (#app #n:_) (il: eac_log app n)
+  : Lemma (ensures (let rs = GI.appfn_calls #(high_verifier_spec app) #n il in
+                    True))
+*)
+  //Zeta.AppSimulate.valid_call_result (appfn_calls il)))
